LiqLeanPolicy/Basic.lean
@@ -1,35 +1,25 @@
 -- Basic Account model for the Liq wallet
 
 -- Address is a 32 byte hex value
-structure Address where
-  value : String
-  deriving DecidableEq, Repr
-
- instance : ToString Address where
-  toString a := a.value
-
+def Address : Type := String
 -- A Liquefaction Account is a shared Account for a group of users
 -- Also known as a "domain". The Account.address is the root address of the Account.
 structure Account where
   address : Address
   owner : Address
-  deriving DecidableEq, Repr
 
 structure SubAccount where
   domain : Account -- The domain or account that this subaccount belongs to
   identifier : String -- The identifier of the subaccount
-  deriving DecidableEq, Repr
 
 -- External Transfer
 structure ExternalTransfer where
   fromAccount : Account
   toAddress : Address -- The address of the external user receiving the funds
   amount : Nat
-  deriving DecidableEq, Repr
 
 -- Internal Transfer
 structure InternalTransfer where
   fromSubAccount : SubAccount
   toSubAccount : SubAccount
   amount : Nat
-  deriving DecidableEq, Repr
